# A.4: Rational Expressions

## Domain of an Algebraic Expression

The *domain* of an algebraic expression is the set of real numbers where an algebraic expression is defined.  This may be all real numbers ($\mathbb{R}$) or may have some range that is not defined.

* The key is to see if there are values of $x$ (or whatever other variable you have) where, if you plug that value into the expression, you won't get a real solution.

> ### Examples
>
> Find the domain of
>
> 1. $4x^3 + 3$
> 2. $\sqrt{x+7}$
> 3. $\displaystyle \frac{x+5}{x}$
>
> <details><summary>Answers</summary><ol><li>In this case, since there is a solution for any real number, the domain is the set of all real numbers</li><li>Here, since we only get a real square root of a number if whatever is under the radical is greater than zero, the domain has to be <math><mrow><mi>x</mi><mo>≥</mo></mrow><mrow><mo form="prefix" stretchy="false">−</mo></mrow><mrow><mn>7</mn></mrow></math></li><li>Here, any x value would work as long as we don't divide by zero, so the domain is <math><mrow><mi>x</mi><mo>≠</mo></mrow><mrow><mn>0</mn></mrow></math></li></ol></details>

> ### Class Question
>
> By factoring the denominator, find the domain for $\displaystyle \frac{x-6}{x^2-49}$.
>
> <details><summary>Answer</summary>Factorizing this, we would get <math><mfrac><mrow><mi>x</mi><mo>−</mo><mn>6</mn></mrow><mrow><mo form="prefix" stretchy="false" lspace="0em" rspace="0em">(</mo><mi>x</mi><mo>+</mo><mn>7</mn><mo form="postfix" stretchy="false">)</mo><mo form="prefix" stretchy="false">(</mo><mi>x</mi><mo>−</mo><mn>7</mn><mo form="postfix" stretchy="false" lspace="0em" rspace="0em">)</mo></mrow></mfrac></math>.  The key is to identify the numbers where the denominator would be zero.  Therefore, the domain is <math><mrow><mi>x</mi><mo>≠</mo></mrow><mrow><mn>7</mn><mo separator="true">,</mo></mrow><mrow><mi>x</mi><mo>≠</mo></mrow><mrow><mo form="prefix" stretchy="false">−</mo></mrow><mrow><mn>7</mn></mrow></math>
> </details>

## Simplifying a Rational Expression

Recall that a fraction is simplest when a numerator and denominator have no common factors.  The key here is to be able to *factor* the expressions in the numerator and denominator so you can identify common factors.

> ### Example
>
> Simplify $\displaystyle \frac{4x+12}{x^2 - 3x-18}$.
>
> <details><summary>Answer</summary><math><mrow><mfrac><mrow><mn>4</mn><mo form="prefix" stretchy="false">(</mo><mi>x</mi><mo>+</mo><mn>3</mn><mo form="postfix" stretchy="false" lspace="0em" rspace="0em">)</mo></mrow><mrow><mo form="prefix" stretchy="false" lspace="0em" rspace="0em">(</mo><mi>x</mi><mo>−</mo><mn>6</mn><mo form="postfix" stretchy="false">)</mo><mo form="prefix" stretchy="false">(</mo><mi>x</mi><mo>+</mo><mn>3</mn><mo form="postfix" stretchy="false" lspace="0em" rspace="0em">)</mo></mrow></mfrac><mo>=</mo></mrow><mrow><mfrac><mn>4</mn><mrow><mi>x</mi><mo>−</mo><mn>6</mn></mrow></mfrac></mrow></math></details>

> ### Class Question
>
> Simplify $\displaystyle \frac{3x+2}{15x^2+22x+8}$
>
> <details><summary>Answer</summary><math><mrow><mfrac><mrow><mn>3</mn><mi>x</mi><mo>+</mo><mn>2</mn></mrow><mrow><mo form="prefix" stretchy="false" lspace="0em" rspace="0em">(</mo><mn>3</mn><mi>x</mi><mo>+</mo><mn>2</mn><mo form="postfix" stretchy="false">)</mo><mo form="prefix" stretchy="false">(</mo><mn>5</mn><mi>x</mi><mo>+</mo><mn>4</mn><mo form="postfix" stretchy="false" lspace="0em" rspace="0em">)</mo></mrow></mfrac><mo>=</mo></mrow><mrow><mfrac><mn>1</mn><mrow><mn>5</mn><mi>x</mi><mo>+</mo><mn>4</mn></mrow></mfrac></mrow></math></details>

## Multiplying or Dividing Rational Expressions

* Factorize the different parts of the expressions as much as possible.
* Follow the rules we have learnt for fractions in Appendix A.1.
* Remember that division means flipping the second fraction.

> ### Examples
>
> Evaluate and simplify, noting down restrictions on the domain
>
> 1. $\displaystyle \frac{15x^2+5x}{x^3 - 3x^2 - 18x} \cdot \frac{x^2 - 2x - 15}{3x^2 - 8x-3}$
> 2. $\displaystyle \frac{x^3-1}{x^2-1} ÷ \frac{x^2+x+1}{x^2+2x+1}$
>
> <details><summary>Answer to Q. 1</summary>The key here is to remember to factorize each of the four parts (the numerator and denominator to each fraction).  Now, <math display="block" class="tml-display" style="display:block math;"><mrow><mfrac><mrow><mn>5</mn><mi>x</mi><mo form="prefix" stretchy="false">(</mo><mn>3</mn><mi>x</mi><mo>+</mo><mn>1</mn><mo form="postfix" stretchy="false" lspace="0em" rspace="0em">)</mo></mrow><mrow><mi>x</mi><mo form="prefix" stretchy="false">(</mo><msup><mi>x</mi><mn class="tml-sml-pad">2</mn></msup><mo>−</mo><mn>3</mn><mi>x</mi><mo>−</mo><mn>18</mn><mo form="postfix" stretchy="false" lspace="0em" rspace="0em">)</mo></mrow></mfrac><mo>⋅</mo><mfrac><mrow><mo form="prefix" stretchy="false" lspace="0em" rspace="0em">(</mo><mi>x</mi><mo>+</mo><mn>3</mn><mo form="postfix" stretchy="false">)</mo><mo form="prefix" stretchy="false">(</mo><mi>x</mi><mo>−</mo><mn>5</mn><mo form="postfix" stretchy="false" lspace="0em" rspace="0em">)</mo></mrow><mrow><mo form="prefix" stretchy="false" lspace="0em" rspace="0em">(</mo><mn>3</mn><mi>x</mi><mo>+</mo><mn>1</mn><mo form="postfix" stretchy="false">)</mo><mo form="prefix" stretchy="false">(</mo><mi>x</mi><mo>−</mo><mn>3</mn><mo form="postfix" stretchy="false" lspace="0em" rspace="0em">)</mo></mrow></mfrac><mo>=</mo><mfrac><mrow><mn>5</mn><mo form="prefix" stretchy="false">(</mo><mn>3</mn><mi>x</mi><mo>+</mo><mn>1</mn><mo form="postfix" stretchy="false" lspace="0em" rspace="0em">)</mo></mrow><mrow><mo form="prefix" stretchy="false" lspace="0em" rspace="0em">(</mo><mi>x</mi><mo>+</mo><mn>3</mn><mo form="postfix" stretchy="false">)</mo><mo form="prefix" stretchy="false">(</mo><mi>x</mi><mo>−</mo><mn>6</mn><mo form="postfix" stretchy="false" lspace="0em" rspace="0em">)</mo></mrow></mfrac><mo>⋅</mo><mfrac><mrow><mo form="prefix" stretchy="false" lspace="0em" rspace="0em">(</mo><mi>x</mi><mo>+</mo><mn>3</mn><mo form="postfix" stretchy="false">)</mo><mo form="prefix" stretchy="false">(</mo><mi>x</mi><mo>−</mo><mn>5</mn><mo form="postfix" stretchy="false" lspace="0em" rspace="0em">)</mo></mrow><mrow><mo form="prefix" stretchy="false" lspace="0em" rspace="0em">(</mo><mn>3</mn><mi>x</mi><mo>+</mo><mn>1</mn><mo form="postfix" stretchy="false">)</mo><mo form="prefix" stretchy="false">(</mo><mi>x</mi><mo>−</mo><mn>3</mn><mo form="postfix" stretchy="false" lspace="0em" rspace="0em">)</mo></mrow></mfrac></mrow></math>.  It is important to note here when we look at the domain on the second step that we cancelled out x from the top and the bottom.  However, this is only possible if <math><mrow><mi>x</mi><mo>≠</mo></mrow><mrow><mn>0</mn></mrow></math>, which we will need to remember for the purpose of knowing what the domain is.  In any event, we now cancel out the terms that are the same on the top and bottom, and we get <math display="block" class="tml-display" style="display:block math;"><mfrac><mrow><mn>5</mn><mo form="prefix" stretchy="false">(</mo><mi>x</mi><mo>−</mo><mn>5</mn><mo form="postfix" stretchy="false" lspace="0em" rspace="0em">)</mo></mrow><mrow><mo form="prefix" stretchy="false" lspace="0em" rspace="0em">(</mo><mi>x</mi><mo>−</mo><mn>3</mn><mo form="postfix" stretchy="false">)</mo><mo form="prefix" stretchy="false">(</mo><mi>x</mi><mo>−</mo><mn>6</mn><mo form="postfix" stretchy="false" lspace="0em" rspace="0em">)</mo></mrow></mfrac></math></details>
>
> <details><summary>Answer to Q. 2</summary>We start by flipping the second fraction, so we have<math display="block" class="tml-display" style="display:block math;"><mrow><mfrac><mrow><msup><mi>x</mi><mn class="tml-sml-pad">3</mn></msup><mo>−</mo><mn>1</mn></mrow><mrow><msup><mi>x</mi><mn class="tml-sml-pad">2</mn></msup><mo>−</mo><mn>1</mn></mrow></mfrac><mo>×</mo><mfrac><mrow><msup><mi>x</mi><mn class="tml-sml-pad">2</mn></msup><mo>+</mo><mn>2</mn><mi>x</mi><mo>+</mo><mn>1</mn></mrow><mrow><msup><mi>x</mi><mn class="tml-sml-pad">2</mn></msup><mo>+</mo><mi>x</mi><mo>+</mo><mn>1</mn></mrow></mfrac></mrow></math>.  Now,  we factorize each term, so we have (making sure we remember our special fractions)<math display="block" class="tml-display" style="display:block math;"><mrow><mfrac><mrow><mo form="prefix" stretchy="false" lspace="0em" rspace="0em">(</mo><mi>x</mi><mo>−</mo><mn>1</mn><mo form="postfix" stretchy="false">)</mo><mo form="prefix" stretchy="false">(</mo><msup><mi>x</mi><mn class="tml-sml-pad">2</mn></msup><mo>+</mo><mi>x</mi><mo>+</mo><mn>1</mn><mo form="postfix" stretchy="false" lspace="0em" rspace="0em">)</mo></mrow><mrow><mo form="prefix" stretchy="false" lspace="0em" rspace="0em">(</mo><mi>x</mi><mo>+</mo><mn>1</mn><mo form="postfix" stretchy="false">)</mo><mo form="prefix" stretchy="false">(</mo><mi>x</mi><mo>−</mo><mn>1</mn><mo form="postfix" stretchy="false" lspace="0em" rspace="0em">)</mo></mrow></mfrac><mo>⋅</mo><mfrac><mrow><mo form="prefix" stretchy="false" lspace="0em" rspace="0em">(</mo><mi>x</mi><mo>+</mo><mn>1</mn><msup><mo form="postfix" stretchy="false">)</mo><mn>2</mn></msup></mrow><mrow><msup><mi>x</mi><mn class="tml-sml-pad">2</mn></msup><mo>+</mo><mi>x</mi><mo>+</mo><mn>1</mn></mrow></mfrac><mo>=</mo><mi>x</mi><mo>+</mo><mn>1</mn></mrow></math>The messy part here is actually figuring out the domain, since we had to cancel out both (x+1) and (x-1) from both sides, so the domain is <math><mrow><mi>x</mi><mo>≠</mo></mrow><mrow><mo form="prefix" stretchy="false">±</mo></mrow><mrow><mn>1</mn></mrow></math>.  (You can show that <math><mrow><msup><mi>x</mi><mn class="tml-sml-pad">2</mn></msup><mo>+</mo></mrow><mrow><mi>x</mi><mo>+</mo></mrow><mrow><mn>1</mn><mo>=</mo></mrow><mrow><mn>0</mn></mrow></math> has no real solution)

> ### Class Question
>
> Evaluate and simplify $\displaystyle \frac{5x}{10x+5}\cdot \frac{14x+7}{3}$.
>
> <details><summary>Answer</summary><math><mrow><mfrac><mrow><mn>5</mn><mi>x</mi></mrow><mrow><mn>5</mn><mo form="prefix" stretchy="false">(</mo><mn>2</mn><mi>x</mi><mo>+</mo><mn>1</mn><mo form="postfix" stretchy="false" lspace="0em" rspace="0em">)</mo></mrow></mfrac><mfrac><mrow><mn>7</mn><mo form="prefix" stretchy="false">(</mo><mn>2</mn><mi>x</mi><mo>+</mo><mn>1</mn><mo form="postfix" stretchy="false" lspace="0em" rspace="0em">)</mo></mrow><mn>3</mn></mfrac><mo>=</mo></mrow><mrow><mfrac><mrow><mn>7</mn><mi>x</mi></mrow><mn>3</mn></mfrac></mrow></math></details>

## Adding or Subtracting Rational Expressions

The key here is to make sure you have a *common denominator* before you add or subtract.  Two ways to do this:

* Find the lowest common denominator
* Multiply together the denominators and cross multiply such that $$\displaystyle \begin{equation}\frac{a}{b} \pm \frac{c}{d} = \frac{ad \pm bc}{bd}\end{equation}$$

> ### Example
>
> Solve for
>
> 1. $\displaystyle \frac{x}{2x-1}-\frac{1}{x+2}$
> 2. $\displaystyle \frac{4}{x} - \frac{x+5}{x^2-4}+\frac{4}{x+2}$
>
> <details><summary>Answer to Q. 1</summary><math display="block" class="tml-display" style="display:block math;"><mrow><mfrac><mrow><mi>x</mi><mo form="prefix" stretchy="false">(</mo><mi>x</mi><mo>+</mo><mn>2</mn><mo form="postfix" stretchy="false">)</mo><mo>−</mo><mo form="prefix" stretchy="false">(</mo><mn>2</mn><mi>x</mi><mo>−</mo><mn>1</mn><mo form="postfix" stretchy="false" lspace="0em" rspace="0em">)</mo></mrow><mrow><mo form="prefix" stretchy="false" lspace="0em" rspace="0em">(</mo><mn>2</mn><mi>x</mi><mo>−</mo><mn>1</mn><mo form="postfix" stretchy="false">)</mo><mo form="prefix" stretchy="false">(</mo><mi>x</mi><mo>+</mo><mn>2</mn><mo form="postfix" stretchy="false" lspace="0em" rspace="0em">)</mo></mrow></mfrac><mo>=</mo><mfrac><mrow><msup><mi>x</mi><mn class="tml-sml-pad">2</mn></msup><mo>+</mo><mn>2</mn><mi>x</mi><mo>−</mo><mn>2</mn><mi>x</mi><mo>+</mo><mn>1</mn></mrow><mrow><mo form="prefix" stretchy="false" lspace="0em" rspace="0em">(</mo><mi>x</mi><mo>+</mo><mn>2</mn><mo form="postfix" stretchy="false">)</mo><mo form="prefix" stretchy="false">(</mo><mn>2</mn><mi>x</mi><mo>−</mo><mn>1</mn><mo form="postfix" stretchy="false" lspace="0em" rspace="0em">)</mo></mrow></mfrac><mo>=</mo><mfrac><mrow><msup><mi>x</mi><mn class="tml-sml-pad">2</mn></msup><mo>+</mo><mn>1</mn></mrow><mrow><mo form="prefix" stretchy="false" lspace="0em" rspace="0em">(</mo><mi>x</mi><mo>+</mo><mn>2</mn><mo form="postfix" stretchy="false">)</mo><mo form="prefix" stretchy="false">(</mo><mn>2</mn><mi>x</mi><mo>−</mo><mn>1</mn><mo form="postfix" stretchy="false" lspace="0em" rspace="0em">)</mo></mrow></mfrac></mrow></math></details>
>
> <details><summary>Answer to Q. 2</summary>Here, it may be very helpful to start by finding the lowest common denominator.  To do this, we start by factorizing the denominator of the second term, so we get <math display="block" class="tml-display" style="display:block math;"><mrow><mfrac><mn>4</mn><mi>x</mi></mfrac><mo>−</mo><mfrac><mrow><mi>x</mi><mo>+</mo><mn>5</mn></mrow><mrow><mo form="prefix" stretchy="false" lspace="0em" rspace="0em">(</mo><mi>x</mi><mo>+</mo><mn>2</mn><mo form="postfix" stretchy="false">)</mo><mo form="prefix" stretchy="false">(</mo><mi>x</mi><mo>−</mo><mn>2</mn><mo form="postfix" stretchy="false" lspace="0em" rspace="0em">)</mo></mrow></mfrac><mo>+</mo><mfrac><mn>4</mn><mrow><mi>x</mi><mo>+</mo><mn>2</mn></mrow></mfrac></mrow></math>We now recognize that the lowest common denominator is <math><mrow><mi>x</mi><mo form="prefix" stretchy="false">(</mo><mi>x</mi><mo>+</mo><mn>2</mn><mo form="postfix" stretchy="false">)</mo><mo form="prefix" stretchy="false">(</mo><mi>x</mi><mo>−</mo><mn>2</mn><mo form="postfix" stretchy="false">)</mo></mrow></math>, so <math display="block" class="tml-display" style="display:block math;"><mrow><mfrac><mrow><mn>4</mn><mo form="prefix" stretchy="false">(</mo><mi>x</mi><mo>+</mo><mn>2</mn><mo form="postfix" stretchy="false">)</mo><mo form="prefix" stretchy="false">(</mo><mi>x</mi><mo>−</mo><mn>2</mn><mo form="postfix" stretchy="false">)</mo><mo>−</mo><mi>x</mi><mo form="prefix" stretchy="false">(</mo><mi>x</mi><mo>+</mo><mn>5</mn><mo form="postfix" stretchy="false">)</mo><mo>+</mo><mn>4</mn><mo form="prefix" stretchy="false">(</mo><mi>x</mi><mo form="postfix" stretchy="false">)</mo><mo form="prefix" stretchy="false">(</mo><mi>x</mi><mo>−</mo><mn>2</mn><mo form="postfix" stretchy="false" lspace="0em" rspace="0em">)</mo></mrow><mrow><mi>x</mi><mo form="prefix" stretchy="false">(</mo><mi>x</mi><mo>+</mo><mn>2</mn><mo form="postfix" stretchy="false">)</mo><mo form="prefix" stretchy="false">(</mo><mi>x</mi><mo>−</mo><mn>2</mn><mo form="postfix" stretchy="false" lspace="0em" rspace="0em">)</mo></mrow></mfrac><mo>=</mo><mfrac><mrow><mn>7</mn><msup><mi>x</mi><mn class="tml-sml-pad">2</mn></msup><mo>−</mo><mn>13</mn><mi>x</mi><mo>−</mo><mn>16</mn></mrow><mrow><mi>x</mi><mo form="prefix" stretchy="false">(</mo><mi>x</mi><mo>+</mo><mn>2</mn><mo form="postfix" stretchy="false">)</mo><mo form="prefix" stretchy="false">(</mo><mi>x</mi><mo>−</mo><mn>2</mn><mo form="postfix" stretchy="false" lspace="0em" rspace="0em">)</mo></mrow></mfrac></mrow></math></details>

> ### Class Question
>
> Solve $\displaystyle \frac{x^2  + 11}{x^2-4x-32}+\frac{5x-7}{x^2-4x-32}$
>
> <details><summary>Answer</summary>The key to this problem is that while they kindly gave you a common denominator, you ultimately still have to factor both the numerator and denominator.  So<math display="block" class="tml-display" style="display:block math;"><mrow><mfrac><mrow><mo form="prefix" stretchy="false" lspace="0em" rspace="0em">(</mo><msup><mi>x</mi><mn class="tml-sml-pad">2</mn></msup><mo>+</mo><mn>11</mn><mo form="postfix" stretchy="false">)</mo><mo>+</mo><mo form="prefix" stretchy="false">(</mo><mn>5</mn><mi>x</mi><mo>−</mo><mn>7</mn><mo form="postfix" stretchy="false" lspace="0em" rspace="0em">)</mo></mrow><mrow><msup><mi>x</mi><mn class="tml-sml-pad">2</mn></msup><mo>−</mo><mn>4</mn><mi>x</mi><mo>−</mo><mn>32</mn></mrow></mfrac><mo>=</mo><mfrac><mrow><msup><mi>x</mi><mn class="tml-sml-pad">2</mn></msup><mo>+</mo><mn>5</mn><mi>x</mi><mo>+</mo><mn>4</mn></mrow><mrow><msup><mi>x</mi><mn class="tml-sml-pad">2</mn></msup><mo>−</mo><mn>4</mn><mi>x</mi><mo>−</mo><mn>32</mn></mrow></mfrac><mo>=</mo><mfrac><mrow><mo form="prefix" stretchy="false" lspace="0em" rspace="0em">(</mo><mi>x</mi><mo>+</mo><mn>4</mn><mo form="postfix" stretchy="false">)</mo><mo form="prefix" stretchy="false">(</mo><mi>x</mi><mo>+</mo><mn>1</mn><mo form="postfix" stretchy="false" lspace="0em" rspace="0em">)</mo></mrow><mrow><mo form="prefix" stretchy="false" lspace="0em" rspace="0em">(</mo><mi>x</mi><mo>+</mo><mn>4</mn><mo form="postfix" stretchy="false">)</mo><mo form="prefix" stretchy="false">(</mo><mi>x</mi><mo>−</mo><mn>8</mn><mo form="postfix" stretchy="false" lspace="0em" rspace="0em">)</mo></mrow></mfrac><mo>=</mo><mfrac><mrow><mi>x</mi><mo>+</mo><mn>1</mn></mrow><mrow><mi>x</mi><mo>−</mo><mn>8</mn></mrow></mfrac></mrow></math></details>

## Complex Fractions

A complex fraction is one where there are separate fractions in the numerator, denominator or both, such as

* $\displaystyle \frac{(\frac{1}{x})}{x^2+1}$
* $\displaystyle \frac{(\frac{1}{x})}{(\frac{1}{x^2+1})}$

The key to solving these is to start by reassembling it as a division problem (as we did above) and then factor/simplify as normal.

> ### Example
>
> Simplify $\displaystyle \frac{\frac{1}{x+2}+1}{\frac{x}{3}-1}$
>
> <details><summary>Answer</summary><math display="block" class="tml-display" style="display:block math;"><mrow><mfrac><mrow><mn>1</mn><mo>+</mo><mo form="prefix" stretchy="false">(</mo><mi>x</mi><mo>+</mo><mn>2</mn><mo form="postfix" stretchy="false" lspace="0em" rspace="0em">)</mo></mrow><mrow><mi>x</mi><mo>+</mo><mn>2</mn></mrow></mfrac><mo>÷</mo><mfrac><mrow><mi>x</mi><mo>−</mo><mn>3</mn></mrow><mn>3</mn></mfrac><mo>=</mo><mfrac><mrow><mi>x</mi><mo>+</mo><mn>3</mn></mrow><mrow><mi>x</mi><mo>+</mo><mn>2</mn></mrow></mfrac><mo>⋅</mo><mfrac><mn>3</mn><mrow><mi>x</mi><mo>−</mo><mn>3</mn></mrow></mfrac><mo>=</mo><mfrac><mrow><mn>3</mn><mo form="prefix" stretchy="false">(</mo><mi>x</mi><mo>+</mo><mn>3</mn><mo form="postfix" stretchy="false" lspace="0em" rspace="0em">)</mo></mrow><mrow><mo form="prefix" stretchy="false" lspace="0em" rspace="0em">(</mo><mi>x</mi><mo>+</mo><mn>2</mn><mo form="postfix" stretchy="false">)</mo><mo form="prefix" stretchy="false">(</mo><mi>x</mi><mo>−</mo><mn>3</mn><mo form="postfix" stretchy="false" lspace="0em" rspace="0em">)</mo></mrow></mfrac></mrow></math></details>

> ### Class Question
>
> Simplify $\displaystyle \frac{4+\frac{2}{x}}{\frac{x}{4} + \frac{1}{8}}$
>
> <details><summary>Answer</summary><math display="block" class="tml-display" style="display:block math;"><mrow><mfrac><mrow><mn>4</mn><mi>x</mi><mo>+</mo><mn>2</mn></mrow><mi>x</mi></mfrac><mo>÷</mo><mfrac><mrow><mn>2</mn><mi>x</mi><mo>+</mo><mn>1</mn></mrow><mn>8</mn></mfrac><mo>=</mo><mfrac><mrow><mn>2</mn><mo form="prefix" stretchy="false">(</mo><mn>2</mn><mi>x</mi><mo>+</mo><mn>1</mn><mo form="postfix" stretchy="false" lspace="0em" rspace="0em">)</mo></mrow><mi>x</mi></mfrac><mo>×</mo><mfrac><mn>8</mn><mrow><mn>2</mn><mi>x</mi><mo>+</mo><mn>1</mn></mrow></mfrac><mo>=</mo><mfrac><mn>16</mn><mi>x</mi></mfrac></mrow></math></details>

## More Complex Problems

We can use similar techniques for negative exponents and radicals.  Note that one way to address negative exponents is to factor out the common factor with the *lesser* exponent.

> ### Example
>
> Simplify $(x-1)^{-1/3}-x(x-1)^{-4/3}$
>
> <details><summary>Answer</summary> The crux to this is to recognize that the lowest common factor is <math><mrow><mo form="prefix" stretchy="false">(</mo><mi>x</mi><mo>−</mo><mn>1</mn><msup><mo form="postfix" stretchy="false">)</mo><mrow><mo lspace="0em" rspace="0em">−</mo><mn>4</mn><mi>/</mi><mn>3</mn></mrow></msup></mrow></math>, and therefore factoring by this factor<math display="block" class="tml-display" style="display:block math;"><mrow><mo form="prefix" stretchy="false">(</mo><mi>x</mi><mo>−</mo><mn>1</mn><msup><mo form="postfix" stretchy="false">)</mo><mrow><mo lspace="0em" rspace="0em">−</mo><mn>4</mn><mi>/</mi><mn>3</mn></mrow></msup><mo form="prefix" stretchy="false">[</mo><mo form="prefix" stretchy="false">(</mo><mi>x</mi><mo>−</mo><mn>1</mn><msup><mo form="postfix" stretchy="false">)</mo><mrow><mo lspace="0em" rspace="0em">+</mo><mn>3</mn><mi>/</mi><mn>3</mn></mrow></msup><mo>−</mo><mi>x</mi><mo form="postfix" stretchy="false">]</mo><mo>=</mo><mo form="prefix" stretchy="false">(</mo><mi>x</mi><mo>−</mo><mn>1</mn><msup><mo form="postfix" stretchy="false">)</mo><mrow><mo lspace="0em" rspace="0em">−</mo><mn>4</mn><mi>/</mi><mn>3</mn></mrow></msup><mo form="prefix" stretchy="false">(</mo><mi>x</mi><mo>−</mo><mn>1</mn><mo>−</mo><mi>x</mi><mo form="postfix" stretchy="false">)</mo><mo>=</mo><mo form="prefix" stretchy="false">−</mo><mfrac><mn>1</mn><mrow><mo form="prefix" stretchy="false" lspace="0em" rspace="0em">(</mo><mi>x</mi><mo>−</mo><mn>1</mn><msup><mo form="postfix" stretchy="false">)</mo><mrow><mn>4</mn><mi>/</mi><mn>3</mn></mrow></msup></mrow></mfrac></mrow></math>
> </details>

> ### Example
>
> Rewrite the difference quotient $\displaystyle \frac{\sqrt{9+h}-3}{h}$ by rationalizing its numerator.
>
> <details><summary>Answer</summary>The crux to this problem is to write out the conjugate of the numerator, so we multiply top and bottom by <math><mrow><msqrt><mrow><mn>9</mn><mo>+</mo><mi>h</mi></mrow></msqrt><mo>+</mo></mrow><mrow><mn>3</mn></mrow></math>.  Therefore, <math display="block" class="tml-display" style="display:block math;"><mrow><mfrac><mrow><msqrt><mrow><mn>9</mn><mo>+</mo><mi>h</mi></mrow></msqrt><mo>−</mo><mn>3</mn></mrow><mi>h</mi></mfrac><mo>⋅</mo><mfrac><mrow><msqrt><mrow><mn>9</mn><mo>+</mo><mi>h</mi></mrow></msqrt><mo>+</mo><mn>3</mn></mrow><mrow><msqrt><mrow><mn>9</mn><mo>+</mo><mi>h</mi></mrow></msqrt><mo>+</mo><mn>3</mn></mrow></mfrac><mo>=</mo><mfrac><mrow><mo form="prefix" stretchy="false" lspace="0em" rspace="0em">(</mo><mn>9</mn><mo>+</mo><mi>h</mi><mo form="postfix" stretchy="false">)</mo><mo>−</mo><mn>9</mn></mrow><mrow><mi>h</mi><mo form="prefix" stretchy="false">(</mo><msqrt><mrow><mn>9</mn><mo>+</mo><mi>h</mi></mrow></msqrt><mo>+</mo><mn>3</mn><mo form="postfix" stretchy="false" lspace="0em" rspace="0em">)</mo></mrow></mfrac><mo>=</mo><mfrac><mi>h</mi><mrow><mi>h</mi><mo form="prefix" stretchy="false">(</mo><msqrt><mrow><mn>9</mn><mo>+</mo><mi>h</mi></mrow></msqrt><mo>+</mo><mn>3</mn><mo form="postfix" stretchy="false" lspace="0em" rspace="0em">)</mo></mrow></mfrac><mo>=</mo><mfrac><mn>1</mn><mrow><msqrt><mrow><mn>9</mn><mo>+</mo><mi>h</mi></mrow></msqrt><mo>+</mo><mn>3</mn></mrow></mfrac></mrow></math></details>

## Examples Sheet

Answer the following end-of-section problems from section A.4: Q. 12, 16, 28, 38, 46, 72